org.metaborg.lang.pcf/coq/Nabl_pos/aux_lemmas.v
@@ -1,4 +1,7 @@
 Require Import List.
+Require Export Setoid.
+Require Import Program.
+Require Import Relation_Operators.
 
 Lemma Forall2_exists_r {A B : Type} : 
   forall l1 l2 P, 
@@ -22,4 +25,54 @@ Proof.
   exists x.
   destruct H1.
   split; [right; eauto | assumption].
+Qed.
+
+
+Lemma in_nth {A} : forall l (p : A), In p l <-> exists n, nth_error l n = Some p.
+Proof.
+  induction l.
+  unfold In.
+  intros; split; intuition.
+  destruct H.
+  destruct x.
+  simpl in H.
+  discriminate H.
+  simpl in H.
+  discriminate H.
+  intros; split; intros.
+  destruct H.
+  exists 0; simpl; subst; eauto.
+  rewrite IHl in H.
+  destruct H.
+  exists (S x).
+  simpl.
+  eauto.
+  destruct H.
+  destruct x.
+  simpl in H.
+  inversion H; subst; left; eauto.
+  simpl in H.
+  destruct (IHl p).
+  right.
+  apply H1.
+  exists x; eauto.
+Qed.
+
+ (* $(&!@ unbelievable that these aren't in the library! *) 
+Lemma tn1_rtn1: forall {A:Type} (R : relation A) (x y: A), 
+                  clos_trans_n1 A R x y -> clos_refl_trans_n1 A R x y. 
+Proof.
+  intros. induction H. 
+  eapply rtn1_trans; eauto.  eapply rtn1_refl.
+  eapply rtn1_trans with y; eauto. 
+Qed.  
+
+Lemma rtn1_tn1: forall {A:Type} (R: relation A) (x y:A),
+                  clos_refl_trans_n1 A R x y -> x = y \/ clos_trans_n1 A R x y. 
+Proof.
+  induction 1. 
+  intuition.
+  inversion IHclos_refl_trans_n1. 
+  right. subst. econstructor; eauto. 
+  right. subst. eapply tn1_trans; eauto. 
 Qed.
